chore: builds

src/Std/Tactic/BVDecide/Bitblast/BVExpr/Basic.lean
@@ -146,7 +146,7 @@ inductive BVUnOp where
   /--
   Population count.
   -/
-  | popCnt
+  | popCount
   deriving Hashable, DecidableEq
 
 namespace BVUnOp
@@ -158,7 +158,7 @@ def toString : BVUnOp → String
   | arithShiftRightConst n => s!">>a {n}"
   | reverse => "rev"
   | clz => "clz"
-  | popCnt => "popCnt"
+  | popCount => "popCount"
 
 instance : ToString BVUnOp := ⟨toString⟩
 
@@ -172,7 +172,7 @@ def eval : BVUnOp → (BitVec w → BitVec w)
   | arithShiftRightConst n => (BitVec.sshiftRight · n)
   | reverse =>  BitVec.reverse
   | clz => BitVec.clz
-  | popCnt => BitVec.popCnt
+  | popCount => BitVec.popCount
 
 @[simp] theorem eval_not : eval .not = ((~~~ ·) : BitVec w → BitVec w) := by rfl
 
@@ -192,7 +192,7 @@ theorem eval_arithShiftRightConst : eval (arithShiftRightConst n) = (BitVec.sshi
 
 @[simp] theorem eval_clz : eval .clz = (BitVec.clz : BitVec w → BitVec w) := by rfl
 
-@[simp] theorem eval_popCnt : eval .popCnt = (BitVec.popCnt : BitVec w → BitVec w) := by rfl
+@[simp] theorem eval_popCount : eval .popCount = (BitVec.popCount : BitVec w → BitVec w) := by rfl
 
 end BVUnOp
 
