src/Std/Tactic/BVDecide/Bitblast/BVExpr/Circuit/Impl/Expr.lean
@@ -20,6 +20,7 @@ import Std.Tactic.BVDecide.Bitblast.BVExpr.Circuit.Impl.Operations.Udiv
 import Std.Tactic.BVDecide.Bitblast.BVExpr.Circuit.Impl.Operations.Umod
 import Std.Tactic.BVDecide.Bitblast.BVExpr.Circuit.Impl.Operations.Reverse
 import Std.Tactic.BVDecide.Bitblast.BVExpr.Circuit.Impl.Operations.Clz
+import Std.Tactic.BVDecide.Bitblast.BVExpr.Circuit.Impl.Operations.PopCount
 
 /-!
 This module contains the implementation of a bitblaster for `BitVec` expressions (`BVExpr`).
@@ -231,8 +232,8 @@ where
           apply AIG.LawfulVecOperator.le_size_of_le_aig_size (f := bitblast.blastClz)
           omega
         ⟨⟨res, this⟩, cache.cast (AIG.LawfulVecOperator.le_size (f := bitblast.blastClz) ..)⟩
-      | .popCnt => sorry
-        -- let res := bitblast.blastPopCnt eaig evec
+      | .popCount => sorry
+        -- let res := bitblast.blastPopCount eaig evec
         -- have := by
         --   apply AIG.LawfulVecOperator.le_size_of_le_aig_size (f := bitblast.blastClz)
         --   omega
@@ -353,7 +354,7 @@ theorem go_decl_eq (aig : AIG BVBit) (expr : BVExpr w) (cache : Cache aig) :
       rw [goCache_decl_eq]
       have := (goCache aig expr cache).result.property
       omega
-    | .popCnt => sorry
+    | .popCount => sorry
   · next lhsExpr rhsExpr h =>
     have hl := (goCache aig lhsExpr cache).result.property
     have hr := (goCache (goCache aig lhsExpr cache).1.1.aig rhsExpr (goCache aig lhsExpr cache).cache).result.property
