src/Std/Tactic/BVDecide/Bitblast/BVExpr/Circuit/Lemmas/Expr.lean
@@ -21,7 +21,7 @@ import Std.Tactic.BVDecide.Bitblast.BVExpr.Circuit.Lemmas.Operations.Udiv
 import Std.Tactic.BVDecide.Bitblast.BVExpr.Circuit.Lemmas.Operations.Umod
 import Std.Tactic.BVDecide.Bitblast.BVExpr.Circuit.Lemmas.Operations.Reverse
 import Std.Tactic.BVDecide.Bitblast.BVExpr.Circuit.Lemmas.Operations.Clz
-import Std.Tactic.BVDecide.Bitblast.BVExpr.Circuit.Lemmas.Operations.PopCnt
+import Std.Tactic.BVDecide.Bitblast.BVExpr.Circuit.Lemmas.Operations.PopCount
 import Std.Tactic.BVDecide.Bitblast.BVExpr.Circuit.Impl.Expr
 
 /-!
